try to prove using different slices

code/mlkem/Hacl.Spec.MLkem.Poly.fst
@@ -59,16 +59,23 @@ val add_rq: a:rq -> b:rq -> rq
 let add_rq a b = add #n a b
 
 // T_q is the image of R_q under the Number Theoretic Transform
-let tq = lseq (lpoly 2) 128
+// let tq = lseq (lpoly 2) 128
+let tq = lseq zq 256
 
-let index_tq (t:tq) (i:size_nat{i < 256}) : zq =
-  let p2 = index t (i / 2) in
-  index p2 (i % 2)
+// let index_tq (t:tq) (i:size_nat{i < 256}) : zq =
+//   let p2 = index t (i / 2) in
+//   index p2 (i % 2)
+let index_tq (t:tq) (i:size_nat{i < 256}) : zq = index t i
 
-let upd_tq (t:tq) (i:size_nat{i < 256}) (v:zq) : tq =
-  let p2 = index t (i / 2) in
-  let p2_upd = upd p2 (i % 2) v in
-  upd t (i / 2) p2_upd
+// let upd_tq (t:tq) (i:size_nat{i < 256}) (v:zq) : tq =
+//   let p2 = index t (i / 2) in
+//   let p2_upd = upd p2 (i % 2) v in
+//   upd t (i / 2) p2_upd
+let upd_tq (t:tq) (i:size_nat{i < 256}) (v:zq) : tq = upd t i v
+
+let rq_to_tq (f:rq) = f
+let tq_to_rq (f:tq) = f
+let tq_eq (f g: tq) = Seq.equal f g
 
 val scalar_mul:
     #deg:size_nat
@@ -122,315 +129,371 @@ val mul_quotient_ring:
 let mul_quotient_ring #deg a b =
   createi deg (fun i -> mul_ab_kth_coeff a b i)
 
-let zeta = 17
-let bit7 = lseq bool 7
+// let zeta = 17
+// let bit7 = lseq bool 7
 
-let bitrev7 (bits:bit7): bit7 =
-  createi 7 (fun i -> index bits (6 - i))
+// let bitrev7 (bits:bit7): bit7 =
+//   createi 7 (fun i -> index bits (6 - i))
 
-let bit (b:bool): b:nat{b = 0 || b = 1} = if b then 1 else 0
+// let bit (b:bool): b:nat{b = 0 || b = 1} = if b then 1 else 0
 
-let bit7_v (bits:bit7): r:nat{r < 128} =
-  let r0 = bit (index bits 0) in 
-  let r1 = bit (index bits 1) in
-  let r2 = bit (index bits 2) in
-  let r3 = bit (index bits 3) in
-  let r4 = bit (index bits 4) in
-  let r5 = bit (index bits 5) in
-  let r6 = bit (index bits 6) in
-  r0 + 2 * r1 + 4 * r2 + 8 * r3 + 16 * r4 + 32 * r5 + 64 * r6
+// let bit7_v (bits:bit7): r:nat{r < 128} =
+//   let r0 = bit (index bits 0) in 
+//   let r1 = bit (index bits 1) in
+//   let r2 = bit (index bits 2) in
+//   let r3 = bit (index bits 3) in
+//   let r4 = bit (index bits 4) in
+//   let r5 = bit (index bits 5) in
+//   let r6 = bit (index bits 6) in
+//   r0 + 2 * r1 + 4 * r2 + 8 * r3 + 16 * r4 + 32 * r5 + 64 * r6
 
-let bitrev_ok (bits:bit7): Lemma 
-  (requires True) 
-  (ensures (
-    let rev = bitrev7 bits in
-    forall (i:nat{ i < 7 }). (index bits i = index rev (6 - i))
-  )) = ()
+// let bitrev_ok (bits:bit7): Lemma 
+//   (requires True) 
+//   (ensures (
+//     let rev = bitrev7 bits in
+//     forall (i:nat{ i < 7 }). (index bits i = index rev (6 - i))
+//   )) = ()
 
-let get_bit (bits:nat{ bits < 128}) (i:nat{i < 7}): b:nat{b = 0 || b = 1 } =
-  bits / (pow2 i) % 2
+// let get_bit (bits:nat{ bits < 128}) (i:nat{i < 7}): b:nat{b = 0 || b = 1 } =
+//   bits / (pow2 i) % 2
 
-let bitsequence (i:nat{ i < 128}): bit7 =
-  createi 7 (fun j -> (get_bit i j) = 1)
+// let bitsequence (i:nat{ i < 128}): bit7 =
+//   createi 7 (fun j -> (get_bit i j) = 1)
 
-let bitrev7_int (bits:nat{bits < 128}): result:nat{result < 128} =
-  bit7_v (bitrev7 (bitsequence bits))
+// let bitrev7_int (bits:nat{bits < 128}): result:nat{result < 128} =
+//   bit7_v (bitrev7 (bitsequence bits))
 
-// Types specifying the possible values of the length and start parameters
-type len_t = l:nat{l = 2 || l = 4 || l = 8 || l = 16 || l = 32 || l = 64 || l = 128}
-type start_t (len:len_t) = s:nat{s % (2*len) = 0 && s < 256}
+// // Types specifying the possible values of the length and start parameters
+// type len_t = l:nat{l = 2 || l = 4 || l = 8 || l = 16 || l = 32 || l = 64 || l = 128}
+// type start_t (len:len_t) = s:nat{s % (2*len) = 0 && s < 256}
 
-// These just convert between the two representations of polynomials, such that 
-// f[2i] = p[i][0] and f[2i+1] = p[i][1] (does not do the actual NTT)
-let rq_to_tq (f:rq): tq =
-  createi 128 (fun i ->
-    let f0 = index f (2 * i) in
-    let f1 = index f (2 * i + 1) in
-    let p: lpoly 2 = cons f0 (cons f1 empty) in
-    p
-  )
-let tq_to_rq (f:tq): rq =
-  createi 256 (fun i ->
-    let p = index f (i / 2) in
-    if i % 2 = 0 then
-      index p 0
-    else
-      index p 1
-  )
-let tq_eq (f g: tq) = 
-  let f_rq = tq_to_rq f in
-  let g_rq = tq_to_rq g in
-  Seq.equal f_rq g_rq
+// // These just convert between the two representations of polynomials, such that 
+// // f[2i] = p[i][0] and f[2i+1] = p[i][1] (does not do the actual NTT)
+// // let rq_to_tq (f:rq): tq =
+// //   createi 128 (fun i ->
+// //     let f0 = index f (2 * i) in
+// //     let f1 = index f (2 * i + 1) in
+// //     let p: lpoly 2 = cons f0 (cons f1 empty) in
+// //     p
+// //   )
+// // let tq_to_rq (f:tq): rq =
+// //   createi 256 (fun i ->
+// //     let p = index f (i / 2) in
+// //     if i % 2 = 0 then
+// //       index p 0
+// //     else
+// //       index p 1
+// //   )
+// // let tq_eq (f g: tq) = 
+// //   let f_rq = tq_to_rq f in
+// //   let g_rq = tq_to_rq g in
+// //   Seq.equal f_rq g_rq
+// let rq_to_tq (f:rq) = f
+// let tq_to_rq (f:tq) = f
+// let tq_eq (f g: tq) = Seq.equal f g
 
-val ntt_inner_inner:
-    z:zq
-  -> f:tq
-  -> j:nat
-  -> len:len_t
-  -> start:start_t len
-  -> Tot (tq) (decreases (start + len) - j)
-let rec ntt_inner_inner z f j len start: tq =
-  // for j <- start; j < start + len; j++
-  if j < (start + len) then
-    // t <- zeta * f_hat[j+ len]
-    let t = mul_zq z (index_tq f (j + len)) in
-    let f_j = index_tq f j in
-    // f_hat[j + len] <- f_hat[j] - t
-    let f_upd = upd_tq f (j + len) (add_zq f_j (neg_zq t)) in
-    // f_hat[j] <- f_hat[j] + t
-    let f_upd_upd = upd_tq f_upd j (add_zq f_j t) in
-    ntt_inner_inner z f_upd_upd (j + 1) len start
-  else
-    f
-
-val zeta_to_k:
-    k:nat{k < 128}
-  -> zq
-let zeta_to_k k = pow_mod #q zeta k
-let test = 
-  let zeta_0 = pow_mod #q zeta 0 in
-  pow_mod_def #q zeta 0;
-  lemma_pow_mod #q zeta 0;
-  lemma_pow0 zeta;
-  assert (zeta_0 = 1);
-  ()
-
-val zeta_to_k_pos_lemma: (k:nat{k > 0 && k < 128}) -> Lemma (requires True) (ensures (zeta_to_k k = mul_zq (zeta_to_k (k - 1)) zeta))
-let zeta_to_k_pos_lemma k = 
-  pow_mod_def #q zeta k;
-  lemma_pow_mod #q zeta k;
-  lemma_pow_unfold zeta k;
-  assert (pow zeta k % q = zeta_to_k k);
-  assert (zeta * pow zeta (k - 1) % q = zeta_to_k k);
-  lemma_pow_mod #q zeta (k - 1);
-  assert (pow zeta (k - 1) % q = zeta_to_k (k - 1));
-  ()
-
-val ntt_outer_inner_body:
-    f:tq
-  -> len:len_t
-  -> start:start_t len
-  -> k:nat{k < 128}
-  -> tq
-let ntt_outer_inner_body f len start k = 
-  // zeta <- Zeta ^ (BitRev7(k)) mod q
-  let z = pow_mod #q zeta (bitrev7_int k) in
-  let f_upd = ntt_inner_inner z f start len start in
-  f_upd
-
-val ntt_outer_inner:
-    f:tq
-  -> len:len_t
-  -> start:start_t len
-  -> Tot (tq) (decreases (256 - 2 * len) - start)
-let rec ntt_outer_inner f len start =
-  let k = (128 / len) + (start / (2 * len)) in
-  let f_upd:tq = ntt_outer_inner_body f len start k in
-  if start + 2 * len >= 256 then 
-    f_upd
-  else
-    ntt_outer_inner f_upd len (start + 2 * len)
-
-val ntt_outer:
-    len:len_t
-  -> f:tq
-  -> Tot tq (decreases len)
-let rec ntt_outer len f =
-  let f_upd = ntt_outer_inner f len 0 in
-  if len = 2 then
-    f_upd
-  else
-    ntt_outer (len / 2) f_upd
-
-let ntt (f:rq): tq =
-  let ntt_image = ntt_outer 128 (rq_to_tq f) in 
-  ntt_image
-
-val intt_inner_inner:
-    z:zq
-  -> f:tq
-  -> j:nat
-  -> len:len_t
-  -> start:start_t len
-  -> Tot (tq) (decreases (start + len) - j)
-let rec intt_inner_inner z f j len start: tq =
-  // for j <- start; j < start + len; j++
-  if j < (start + len) then
-    // t <- zeta * f_hat[j+ len]
-    let t = (index_tq f j) in 
-    // f[j] <- t + f[j+len]
-    let f_j = add_zq t (index_tq f (j + len)) in
-    let f_upd = upd_tq f j f_j in
-    // f[j+len] <- zeta * (f[j+len] - t)
-    let f_j_len = mul_zq z (add_zq (index_tq f (j + len)) (neg_zq t)) in
-    let f_upd_upd = upd_tq f_upd (j + len) f_j_len in
-    intt_inner_inner z f_upd_upd (j + 1) len start
-  else
-    f
-
-val intt_outer_inner_body:
-    f:tq
-  -> len:len_t
-  -> start:start_t len
-  -> k:nat{k < 128}
-  -> tq
-let intt_outer_inner_body f len start k =
-  // zeta <- Zeta ^ (BitRev7(k)) mod q
-  let z = pow_mod #q zeta (bitrev7_int k) in
-  let f_upd = intt_inner_inner z f start len start in
-  f_upd
-
-
-val intt_outer_inner:
-    f:tq
-  -> len:len_t
-  -> start:start_t len
-  -> Tot tq (decreases (256 - 2 * len) - start)
-let rec intt_outer_inner f len start =
-  let k = (256 / len) - (start / (2 * len)) - 1 in
-  // zeta <- Zeta ^ (BitRev7(k)) mod q
-  let z = pow_mod #q zeta (bitrev7_int k) in
-  let f_upd = intt_outer_inner_body f len start k in
-  if start + 2 * len >= 256 then
-    f_upd
-  else
-    intt_outer_inner f_upd len (start + 2 * len)
-
-val intt_outer:
-    len:len_t
-  -> f:tq
-  -> Tot tq (decreases (128 - len))
-let rec intt_outer len f =
-  let f_upd = intt_outer_inner f len 0 in
-  if len = 128 then
-    f_upd
-  else
-    intt_outer (len * 2) f_upd
-
-val intt:
-    f:tq
-  -> rq
-let intt f =
-  let intt_image = intt_outer 128 f in 
-  let unscaled_intt = tq_to_rq intt_image in
-  scalar_mul unscaled_intt 3303
-
-// NTT multiplication specification
-// i-th coordinate in Tq of the product hat(h) = hat(f) x_Tq hat(g) is given by:
-//    hat(h)[2i] + hat(h)[2i+1] = (hat(f)[2i]+hat(f)[2i+1]X) * (hat(g)[2i]+hat(g)[2i+1]X) mod (X^2 - zeta^(2 BitRev_7(i)+1))
-
-// index f i should yield an lpoly 2 which is equivalent to f[2i]+f[2i+1]X
-// ntt_mul_base calculates the product of two lpoly 2 with modulus X^2 - gamma
-let ntt_mul_base (a b:lpoly 2) (gamma: zq): lpoly 2 =
-  let c0 = add_zq (mul_zq (index a 0) (index b 0)) (mul_zq gamma (mul_zq (index a 1) (index b 1))) in
-  let c1 = add_zq (mul_zq (index a 0) (index b 1)) (mul_zq (index a 1) (index b 0)) in
-  cons c0 (cons c1 empty)
-
-val ntt_mul:
-    f:tq
-  -> g:tq
-  -> tq 
-let ntt_mul f g =
-  createi 128 (fun i -> 
-    let gamma = pow_mod #q zeta ((2 * bit7_v (bitrev7 (bitsequence i))) + 1) in
-    ntt_mul_base (index f i) (index g i) gamma
-    )
-
-val ntt_mul_ok:
-    f:rq
-  -> g:rq
-  -> Lemma (requires True) (ensures (intt (ntt_mul (ntt f) (ntt g)) = mul_quotient_ring f g))
-
-
-// NTT correctness specification.
-// hat(f) := (f mod (X^2 - zeta^(2 BitRev_7(0)+1)), ... , f mod (X^2 - zeta^(2 BitRev_7(127)+1)))
-// val ntt:
-//     a:rq
-//   -> Pure (tq) (requires True) (ensures (fun r -> r = a))
-
-
-// val prev_step:
-//     deg:size_nat
-//   -> i:int{ 0 <= i && i < deg}
-//   -> j:int{ 0 <= j && j < deg}
-//   -> tuple2 int int
-// let prev_step deg i j =
-//   if j = 0 then
-//     (i - 1, deg - 1)
+// val ntt_inner_inner:
+//     z:zq
+//   -> f:tq
+//   -> j:nat
+//   -> len:len_t
+//   -> start:start_t len
+//   -> Tot (tq) (decreases (start + len) - j)
+// let rec ntt_inner_inner z f j len start: tq =
+//   // for j <- start; j < start + len; j++
+//   if j < (start + len) then
+//     // t <- zeta * f_hat[j+ len]
+//     let t = mul_zq z (index_tq f (j + len)) in
+//     let f_j = index_tq f j in
+//     // f_hat[j + len] <- f_hat[j] - t
+//     let f_upd = upd_tq f (j + len) (add_zq f_j (neg_zq t)) in
+//     // f_hat[j] <- f_hat[j] + t
+//     let f_upd_upd = upd_tq f_upd j (add_zq f_j t) in
+//     ntt_inner_inner z f_upd_upd (j + 1) len start
 //   else
-//     (i, j - 1)
+//     f
 
-// val mul_intermediate:
-//     #deg:size_nat
-//   -> a:lpoly deg
-//   -> b:lpoly deg
-//   -> i:int{ 0 <= i && i < deg}
-//   -> j:int{ 0 <= j && j < deg}
-//   -> lpoly deg
-// let rec mul_intermediate #deg a b i j =
-//   let c = mul_zq (index a i) (index b j) in
-//   if i + j = 0 then 
-//     let res = create deg 0 in
-//     upd res 0 c
+// val ntt_inner_inner_f (j:nat{j < 256}) (len:len_t) (start:start_t len) (z:zq) (f:tq): zq
+// let ntt_inner_inner_f j len start z f =
+//     if j < start || j >= start + 2 * len then
+//       index_tq f j
+//     else if j >= start && j < start + len then
+//       let t = mul_zq z (index_tq f (j + len)) in
+//       add_zq (index_tq f j) t
+//     else
+//       let t = mul_zq z (index_tq f j) in
+//       add_zq (index_tq f (j - len)) (neg_zq t)
+
+
+// val ntt_inner_inner_func:
+//     z:zq 
+//   -> f:tq 
+//   -> len:len_t
+//   -> start:start_t len
+//   -> tq
+// let ntt_inner_inner_func z f len start = 
+//   let rq_rep = createi #zq 256 (fun j -> ntt_inner_inner_f j len start z f) in rq_to_tq rq_rep
+
+// // val ntt_inner_inner_func_ok: 
+// //     z:zq
+// //   -> f:tq
+// //   -> len:len_t
+// //   -> start:start_t len
+// //   -> Lemma (ensures ntt_inner_inner z f start len start = ntt_inner_inner_func z f len start)
+// // let ntt_inner_inner_func_ok z f len start = ()
+
+// val zeta_to_k:
+//     k:nat{k < 128}
+//   -> zq
+// let zeta_to_k k = pow_mod #q zeta k
+// let test = 
+//   let zeta_0 = pow_mod #q zeta 0 in
+//   pow_mod_def #q zeta 0;
+//   lemma_pow_mod #q zeta 0;
+//   lemma_pow0 zeta;
+//   assert (zeta_0 = 1);
+//   ()
+
+// val zeta_to_k_pos_lemma: (k:nat{k > 0 && k < 128}) -> Lemma (requires True) (ensures (zeta_to_k k = mul_zq (zeta_to_k (k - 1)) zeta))
+// let zeta_to_k_pos_lemma k = 
+//   pow_mod_def #q zeta k;
+//   lemma_pow_mod #q zeta k;
+//   lemma_pow_unfold zeta k;
+//   assert (pow zeta k % q = zeta_to_k k);
+//   assert (zeta * pow zeta (k - 1) % q = zeta_to_k k);
+//   lemma_pow_mod #q zeta (k - 1);
+//   assert (pow zeta (k - 1) % q = zeta_to_k (k - 1));
+//   ()
+
+// val ntt_outer_inner_body:
+//     f:tq
+//   -> len:len_t
+//   -> start:start_t len
+//   -> k:nat{k < 128}
+//   -> tq
+// let ntt_outer_inner_body f len start k = 
+//   // zeta <- Zeta ^ (BitRev7(k)) mod q
+//   let z = pow_mod #q zeta (bitrev7_int k) in
+//   let f_upd = ntt_inner_inner z f start len start in
+//   f_upd
+
+// val ntt_outer_inner:
+//     f:tq
+//   -> len:len_t
+//   -> start:start_t len
+//   -> Tot (tq) (decreases (256 - 2 * len) - start)
+// let rec ntt_outer_inner f len start =
+//   let k = (128 / len) + (start / (2 * len)) in
+//   let f_upd:tq = ntt_outer_inner_body f len start k in
+//   if start + 2 * len >= 256 then 
+//     f_upd
 //   else
-//     let (prev_i, prev_j) = prev_step deg i j in
-//     let res = mul_intermediate a b prev_i prev_j in
-//     upd res ((i + j) % deg) (add_zq c (index res ((i + j) % deg)))
+//     ntt_outer_inner f_upd len (start + 2 * len)
 
-// val mul: 
-//     #deg:size_nat
-//   -> a:lpoly deg
-//   -> b:lpoly deg
-//   -> lpoly deg
-// let mul #deg a b = 
-//   if deg = 0 then 
-//     create 0 0
+// val ntt_outer:
+//     len:len_t
+//   -> f:tq
+//   -> Tot tq (decreases len)
+// let rec ntt_outer len f =
+//   let f_upd = ntt_outer_inner f len 0 in
+//   if len = 2 then
+//     f_upd
 //   else
-//     mul_intermediate a b (deg - 1) (deg - 1)
+//     ntt_outer (len / 2) f_upd
+
+// val len_t_lemma: (i:nat{i < 7}) -> 
+//   Lemma (ensures pow2 i = 2 || pow2 i = 4 || pow2 i = 8 || pow2 i = 16 || pow2 i = 32 || pow2 i = 64)
+// let len_t_lemma i = admit()
+
+// val ntt_outer_intermediate:
+//     f:tq
+//   -> i:nat{i < 7}
+//   -> Tot tq (decreases i)
+// let rec ntt_outer_intermediate f i =
+//   len_t_lemma (6-i);
+//   let len:len_t = 128 / (pow2 (6-i)) in
+//   let f_upd = ntt_outer_inner f len 0 in
+//   if i = 0 then
+//     f_upd
+//   else
+//     ntt_outer_intermediate f_upd (i-1)
+
+// // val ntt_outer_int_ok: 
+// //     f:tq
+// //   -> Lemma (requires True) (ensures (ntt_outer 128 f = ntt_outer_intermediate f 6))
+// // let ntt_outer_int_ok f =
+// //   assert (ntt_outer 2 f = ntt_outer_intermediate f 0);
+// //   ()
+
+// let ntt (f:rq): tq =
+//   let ntt_image = ntt_outer 128 (rq_to_tq f) in 
+//   ntt_image
+
+// val intt_inner_inner:
+//     z:zq
+//   -> f:tq
+//   -> j:nat
+//   -> len:len_t
+//   -> start:start_t len
+//   -> Tot (tq) (decreases (start + len) - j)
+// let rec intt_inner_inner z f j len start: tq =
+//   // for j <- start; j < start + len; j++
+//   if j < (start + len) then
+//     // t <- zeta * f_hat[j+ len]
+//     let t = (index_tq f j) in 
+//     // f[j] <- t + f[j+len]
+//     let f_j = add_zq t (index_tq f (j + len)) in
+//     let f_upd = upd_tq f j f_j in
+//     // f[j+len] <- zeta * (f[j+len] - t)
+//     let f_j_len = mul_zq z (add_zq (index_tq f (j + len)) (neg_zq t)) in
+//     let f_upd_upd = upd_tq f_upd (j + len) f_j_len in
+//     intt_inner_inner z f_upd_upd (j + 1) len start
+//   else
+//     f
+
+// val intt_outer_inner_body:
+//     f:tq
+//   -> len:len_t
+//   -> start:start_t len
+//   -> k:nat{k < 128}
+//   -> tq
+// let intt_outer_inner_body f len start k =
+//   // zeta <- Zeta ^ (BitRev7(k)) mod q
+//   let z = pow_mod #q zeta (bitrev7_int k) in
+//   let f_upd = intt_inner_inner z f start len start in
+//   f_upd
 
 
-let test1 = 
-  let a: lpoly 1 = 
-  let m = mul_zq 1 2 in
-  let res = create 1 0 in 
-  upd res 0 m in
-  assert (index a 0 = 2);
-  assert (length a = 1);
-  assert (Seq.equal a (Seq.cons 2 Seq.empty))
+// val intt_outer_inner:
+//     f:tq
+//   -> len:len_t
+//   -> start:start_t len
+//   -> Tot tq (decreases (256 - 2 * len) - start)
+// let rec intt_outer_inner f len start =
+//   let k = (256 / len) - (start / (2 * len)) - 1 in
+//   // zeta <- Zeta ^ (BitRev7(k)) mod q
+//   let z = pow_mod #q zeta (bitrev7_int k) in
+//   let f_upd = intt_outer_inner_body f len start k in
+//   if start + 2 * len >= 256 then
+//     f_upd
+//   else
+//     intt_outer_inner f_upd len (start + 2 * len)
 
-// val mul_equal_3_: Lemma () 
+// val intt_outer:
+//     len:len_t
+//   -> f:tq
+//   -> Tot tq (decreases (128 - len))
+// let rec intt_outer len f =
+//   let f_upd = intt_outer_inner f len 0 in
+//   if len = 128 then
+//     f_upd
+//   else
+//     intt_outer (len * 2) f_upd
+
+// val intt:
+//     f:tq
+//   -> rq
+// let intt f =
+//   let intt_image = intt_outer 128 f in 
+//   let unscaled_intt = tq_to_rq intt_image in
+//   scalar_mul unscaled_intt 3303
+
+// // NTT multiplication specification
+// // i-th coordinate in Tq of the product hat(h) = hat(f) x_Tq hat(g) is given by:
+// //    hat(h)[2i] + hat(h)[2i+1] = (hat(f)[2i]+hat(f)[2i+1]X) * (hat(g)[2i]+hat(g)[2i+1]X) mod (X^2 - zeta^(2 BitRev_7(i)+1))
+
+// // index f i should yield an lpoly 2 which is equivalent to f[2i]+f[2i+1]X
+// // ntt_mul_base calculates the product of two lpoly 2 with modulus X^2 - gamma
+// let ntt_mul_base (a b:lpoly 2) (gamma: zq): lpoly 2 =
+//   let c0 = add_zq (mul_zq (index a 0) (index b 0)) (mul_zq gamma (mul_zq (index a 1) (index b 1))) in
+//   let c1 = add_zq (mul_zq (index a 0) (index b 1)) (mul_zq (index a 1) (index b 0)) in
+//   cons c0 (cons c1 empty)
+
+// // val ntt_mul:
+// //     f:tq
+// //   -> g:tq
+// //   -> tq 
+// // let ntt_mul f g =
+// //   createi 128 (fun i -> 
+// //     let gamma = pow_mod #q zeta ((2 * bit7_v (bitrev7 (bitsequence i))) + 1) in
+// //     ntt_mul_base (index f i) (index g i) gamma
+// //     )
+
+// // val ntt_mul_ok:
+// //     f:rq
+// //   -> g:rq
+// //   -> Lemma (requires True) (ensures (intt (ntt_mul (ntt f) (ntt g)) = mul_quotient_ring f g))
+
+
+// // NTT correctness specification.
+// // hat(f) := (f mod (X^2 - zeta^(2 BitRev_7(0)+1)), ... , f mod (X^2 - zeta^(2 BitRev_7(127)+1)))
+// // val ntt:
+// //     a:rq
+// //   -> Pure (tq) (requires True) (ensures (fun r -> r = a))
+
+
+// // val prev_step:
+// //     deg:size_nat
+// //   -> i:int{ 0 <= i && i < deg}
+// //   -> j:int{ 0 <= j && j < deg}
+// //   -> tuple2 int int
+// // let prev_step deg i j =
+// //   if j = 0 then
+// //     (i - 1, deg - 1)
+// //   else
+// //     (i, j - 1)
+
+// // val mul_intermediate:
+// //     #deg:size_nat
+// //   -> a:lpoly deg
+// //   -> b:lpoly deg
+// //   -> i:int{ 0 <= i && i < deg}
+// //   -> j:int{ 0 <= j && j < deg}
+// //   -> lpoly deg
+// // let rec mul_intermediate #deg a b i j =
+// //   let c = mul_zq (index a i) (index b j) in
+// //   if i + j = 0 then 
+// //     let res = create deg 0 in
+// //     upd res 0 c
+// //   else
+// //     let (prev_i, prev_j) = prev_step deg i j in
+// //     let res = mul_intermediate a b prev_i prev_j in
+// //     upd res ((i + j) % deg) (add_zq c (index res ((i + j) % deg)))
+
+// // val mul: 
+// //     #deg:size_nat
+// //   -> a:lpoly deg
+// //   -> b:lpoly deg
+// //   -> lpoly deg
+// // let mul #deg a b = 
+// //   if deg = 0 then 
+// //     create 0 0
+// //   else
+// //     mul_intermediate a b (deg - 1) (deg - 1)
+
+
+// let test1 = 
+//   let a: lpoly 1 = 
+//   let m = mul_zq 1 2 in
+//   let res = create 1 0 in 
+//   upd res 0 m in
+//   assert (index a 0 = 2);
+//   assert (length a = 1);
+//   assert (Seq.equal a (Seq.cons 2 Seq.empty))
+
+// // val mul_equal_3_: Lemma () 
   
-#reset-options "--z3rlimit 50 --fuel 0 --ifuel 0"
-let test2 = 
-  let a: lpoly 1 = Seq.cons 1 Seq.empty in
-  let b: lpoly 1 = Seq.cons 3 Seq.empty in
-  let p: lpoly 1 = mul_quotient_ring a b in
-  assert (index p 0 = mul_ab_kth_coeff a b 0)
+// #reset-options "--z3rlimit 50 --fuel 0 --ifuel 0"
+// let test2 = 
+//   let a: lpoly 1 = Seq.cons 1 Seq.empty in
+//   let b: lpoly 1 = Seq.cons 3 Seq.empty in
+//   let p: lpoly 1 = mul_quotient_ring a b in
+//   assert (index p 0 = mul_ab_kth_coeff a b 0)
 
 
-// let a: lpoly 2 = Seq.cons 1 (Seq.cons 2 Seq.empty)
-// let b: lpoly 2 = Seq.cons 3 (Seq.cons 5 Seq.empty)
-// let c: lpoly 2 = mul a b
-// let _ = 
-//   assert (length c = 2);
-//   assert (index c 0 = 11)
+// // let a: lpoly 2 = Seq.cons 1 (Seq.cons 2 Seq.empty)
+// // let b: lpoly 2 = Seq.cons 3 (Seq.cons 5 Seq.empty)
+// // let c: lpoly 2 = mul a b
+// // let _ = 
+// //   assert (length c = 2);
+// //   assert (index c 0 = 11)
