code/mlkem/Hacl.MLkem.NTT.fst
@@ -1,0 +1,618 @@
+module Hacl.MLkem.NTT
+
+open FStar.HyperStack
+open FStar.HyperStack.ST
+open FStar.Mul
+open FStar.Seq
+open FStar.Int
+open Lib.NatMod
+
+module PS = Hacl.Spec.MLkem.Poly
+module B = LowStar.Buffer
+module ST = FStar.HyperStack.ST
+module HS = FStar.HyperStack
+module S = Hacl.Spec.MLkem.NTT
+module Seq = Lib.Sequence
+module M = LowStar.Modifies
+module U32 = FStar.UInt32
+module LE = Lib.Exponentiation
+module PT = Hacl.Impl.PrecompTable
+
+open FStar.Ghost
+open Lib.Buffer
+open Lib.IntTypes
+open Hacl.MLkem.Poly
+// open Lib.Loops
+
+#reset-options "--z3rlimit 50 --fuel 0 --ifuel 0"
+let zeta = u32 S.zeta
+
+// val and_lte_lemma (a b:uint32): Lemma (requires True) (ensures (v (a &. b) <= v a) && (v (a &. b) <= v b))
+// let and_lte_lemma a b =
+//   logand_pos_le #128 (v a) (v b);
+//   logand_spec a b;
+//   ()
+
+// val bitrev7_:
+//     num:U32.t{v num < 128} 
+//   -> (i:size_t{v i <= 6}) 
+//   -> (res:U32.t{v res < 128})
+//   -> Stack U32.t 
+//     (requires fun _ -> Seq.slice (S.bitsequence (v res)) 0 (v i) = Seq.slice (S.bitrev7 (S.bitsequence (v num))) 0 (v i))
+//     (ensures fun _ r _ -> v r < 128 && Seq.slice (S.bitsequence (v r)) 0 ((v i) + 1) = Seq.slice (S.bitrev7 (S.bitsequence (v num))) 0 ((v i) + 1))
+// let rec bitrev7_ num i res =
+//   let mask_low_bit = num &. (1ul) in
+//   let rev_bit = mask_low_bit <<. (6ul -. i) in
+//   let res_upd = res &. rev_bit in
+//   logand_spec res rev_bit;
+//   assert (v (res &. rev_bit) = logand_v (v res) (v rev_bit));
+//   logand_pos_le #128 (v res) (v rev_bit);
+//   if i >=. 6ul then
+//     res_upd
+//   else
+//     bitrev7_ (num >>. 1ul) (i +. 1ul) res_upd
+
+
+// val bitrev7 (num: uint32{v num < 128}): Stack U32.t
+//   (requires fun _ -> True)
+//   (ensures fun _ r _ -> v r < 128 && S.bitsequence (v r) = S.bitrev7 (S.bitsequence (v num)))
+// let bitrev7 num =
+//   admit()
+//   // let rev_spec = S.bit7_v (S.bitrev7 (S.bitsequence (v num))) in
+//   // let res = bitrev7_ num 0ul (u32 0) in
+//   // res
+
+// val z_exp (k:uint32{v k < 128}): uint32
+// let z_exp k = 
+//   admit()
+//   // let rec loop (i:uint32) (acc:uint32): uint32 =
+//   //   if i = k then
+//   //     acc
+//   //   else
+//   //     let acc' = mul_zq acc zeta in
+//   //     loop (i +. 1ul) acc'
+//   // in
+//   // loop 0ul zeta
+
+// let precomp_zeta_table_list: x:list zq{FStar.List.Tot.length x = 128} 
+//   = normalize_term (SPT.precomp_base_table_list )
+// val precomp_zeta_table: x:glbuffer zq 128ul{witnessed x precomp_zeta_table_lseq /\ recallable x}
+// let precomp_zeta_table = createL_global (Seq.to_list precomp_zeta_table_lseq)
+
+val precomp_zeta_lseq : erased (Seq.lseq zq 128)
+let precomp_zeta_lseq =
+  Seq.createi 128 (fun i -> 
+    let z = S.zeta_to_k i in 
+    let z':zq = u32 z in
+    z')
+
+val seq_eq_idx_lemma: #len:size_nat -> s1:lseq zq len -> s2:lseq zq len -> i:nat{i < len} -> Lemma (requires Seq.equal #_ #len s1 s2) (ensures Seq.index #_ #len s1 i == Seq.index #_ #len s2 i)
+let seq_eq_idx_lemma s1 s2 i = ()
+
+let is_zeta_table (table:lbuffer zq 128ul) h = Seq.equal (as_seq h table) precomp_zeta_lseq
+
+val index_zeta_table:
+    i:size_t{i <. 128ul}
+  -> table:lbuffer zq 128ul
+  -> Stack zq 
+    (requires fun h -> live h table /\ is_zeta_table table h)
+    (ensures fun h0 r h1 -> live h1 table /\ zq_v r = S.zeta_to_k (v i))
+let index_zeta_table i table =
+  table.(i)
+
+val precomp_zeta: table:lbuffer zq 128ul -> Stack unit 
+  (requires fun h -> live h table)
+  (ensures fun h0 _ h1 -> live h1 table /\ is_zeta_table table h1)
+let precomp_zeta table = 
+  push_frame ();
+  let h0 = ST.get () in
+  let inv h (i:nat) = 
+    live h table /\
+    modifies (loc table) h0 h /\
+    i <= 128 /\ 
+    Seq.equal (Seq.slice precomp_zeta_lseq 0 i) (Seq.slice (as_seq h table) 0 i) in
+  table.(0ul) <- u32 1;
+  pow_mod_def #PS.q S.zeta 0;
+  lemma_pow_mod #PS.q S.zeta 0;
+  lemma_pow0 S.zeta;
+  assert (S.zeta_to_k 0 == 1);
+  let h' = ST.get () in
+  assert (v (Seq.index (as_seq h' table) 0) == (S.zeta_to_k 0));
+  let body (i: U32.t{1 <= U32.v i && U32.v i < 128}): 
+    Stack unit 
+    (requires fun h -> inv h (U32.v i))
+    (ensures fun h0 _ h1 -> inv h0 (U32.v i) /\ inv h1 (U32.v i + 1)) 
+  =
+    let h0 = ST.get () in
+    let table_as_seq: erased (Seq.lseq zq 128) = as_seq h0 table in
+    assert (Seq.equal (Seq.slice table_as_seq 0 (v i)) (Seq.slice precomp_zeta_lseq 0 (v i)));
+    seq_eq_idx_lemma #(v i) (Seq.slice table_as_seq 0 (v i)) (Seq.slice precomp_zeta_lseq 0 (v i)) (v i - 1);
+    assert ((Seq.index table_as_seq (v i - 1)) == (Seq.index precomp_zeta_lseq (v i - 1)));
+    assert (v (Seq.index precomp_zeta_lseq (v i - 1)) == S.zeta_to_k (v i - 1));
+    assert (v table.(i -. 1ul) == S.zeta_to_k (v i - 1));
+    S.zeta_to_k_pos_lemma (v i);
+    table.(i) <- mul_zq table.(i -. 1ul) zeta;
+    let h1 = ST.get () in
+    assert (v table.(i) == S.zeta_to_k (v i));
+    assert (Seq.index (as_seq h1 table) (v i) == Seq. index precomp_zeta_lseq (v i));
+    assert (Seq.equal (Seq.slice (as_seq h1 table) 0 (v i)) (Seq.slice precomp_zeta_lseq 0 (v i)));
+    slice_plus_one #_ #128 #128 (as_seq h1 table) precomp_zeta_lseq 0 (v i)
+  in
+  Lib.Loops.for 1ul 128ul inv body;
+  pop_frame ()
+
+type len_t = l:size_t{v l = 2 || v l = 4 || v l = 8 || v l = 16 || v l = 32 || v l = 64 || v l = 128}
+type start_t (len:len_t) = s:size_t{v s < 256 && (v s) % (2 * (v len)) = 0}
+val start_plus_len: #len:len_t -> s:start_t len -> Lemma (ensures v s + v len < 256)
+let start_plus_len #len s = ()
+
+val start_t_lemma: 
+    #i:size_t{v i < 7}
+  -> i':size_t{i' <. (1ul <<. i)}
+  -> Lemma (ensures 2 * (v (128ul >>. i)) * (v i' + 1) <= 256)
+let start_t_lemma #i i' =
+  let len = 128ul >>. i in
+  assert (v i' < pow2 (v i));
+  assume (pow2 7 = 128);
+  assert (v len = pow2 7 / pow2 (v i));
+  ()
+
+val ntt_inner_inner_f_ok_1:
+    j:nat
+  -> len:len_t
+  -> start:start_t len
+  -> z:zq
+  -> res_j:zq
+  -> res_j_plus_len:zq
+  -> f:PS.tq
+  -> t:zq
+  -> Lemma 
+      (requires 
+        j < v start + v len /\
+        j >= v start /\
+        v res_j = PS.index_tq f j /\ 
+        j + v len < 256 /\
+        v res_j_plus_len = PS.index_tq f (j + v len) /\ 
+        v t = PS.mul_zq (v z) (v res_j_plus_len)
+      )
+      (ensures v (add_zq res_j t) = S.ntt_inner_inner_f j (v len) (v start) (v z) f)
+let ntt_inner_inner_f_ok_1 j len start z res_j res_j_plus_len f t = ()
+
+val ntt_inner_inner_f_ok_2:
+    j:nat
+  -> len:len_t
+  -> start:start_t len
+  -> z:zq
+  -> res_j:zq
+  -> res_j_minus_len:zq
+  -> f:PS.tq
+  -> t:zq
+  -> Lemma 
+      (requires 
+        j < v start + 2 * (v len) /\
+        j >= v start + v len /\
+        j < 256 /\
+        v res_j = PS.index_tq f j /\ 
+        v res_j_minus_len = PS.index_tq f (j - v len) /\ 
+        v t = PS.mul_zq (v z) (v res_j)
+      )
+      (ensures v (add_zq res_j_minus_len (neg_zq t)) = S.ntt_inner_inner_f j (v len) (v start) (v z) f)
+let ntt_inner_inner_f_ok_2 j len start z res_j res_j_plus_len f t = ()
+
+val seq_slice_idx_lemma:
+    #a:eqtype
+  -> start:nat
+  -> fin:nat{start <= fin /\ fin <= 256}
+  -> i:nat{start <= i /\ i < fin}
+  -> s1:lseq a 256
+  -> s2:lseq a 256
+  -> Lemma 
+      (requires Seq.equal (Seq.slice #_ #256 s1 start fin) (Seq.slice #_ #256 s2 start fin))
+      (ensures Seq.index #a #256 s1 i = Seq.index #a #256 s2 i)
+let seq_slice_idx_lemma #a start fin i s1 s2 =
+  let slice_i = i - start in
+  let slice1 = Seq.slice #_ #256 s1 start fin in
+  let slice2 = Seq.slice #_ #256 s2 start fin in
+  assert (Seq.index slice1 slice_i = Seq.index slice2 slice_i)
+
+#reset-options "--z3rlimit 20 --fuel 0 --ifuel 0"
+
+let inv_inner_inner h0 (z:zq) (len:len_t) (start:start_t len{v start + (2 * v len) <= 256}) (spec_res:erased (lseq PS.zq PS.n)) (res:rq) h (j:nat) =
+    // start_plus_len #len start;
+    live h res /\
+    modifies (loc res) h0 h /\
+    j <= v start + v len /\
+    j >= v start /\
+    j <= 256 /\
+    j >= 0 /\
+    Seq.equal
+      (Seq.slice (lpoly_v h res) j (v start + v len))
+      (Seq.slice (lpoly_v h0 res) j (v start + v len)) /\
+    Seq.equal
+      (Seq.slice (lpoly_v h res) (j + v len) (v start + 2 * (v len)))
+      (Seq.slice (lpoly_v h0 res) (j + v len) (v start + 2 * (v len))) /\
+    Seq.equal 
+      (Seq.slice (lpoly_v h res) (v start) j) 
+      (Seq.slice #_ #(PS.n) spec_res (v start) j) /\
+    Seq.equal 
+      (Seq.slice (lpoly_v h res) (v start + v len) (v len + j))
+      (Seq.slice #_ #(PS.n) spec_res (v start + v len) (v len + j))
+
+let add_v_lemma (a b:U32.t): Lemma (requires v a <= 256 /\ v b <= 256) (ensures v (a +. b) = v a + v b) = ()
+
+val body_inner_inner_1:
+    orig_seq:PS.lpoly PS.n
+  -> old_seq:PS.lpoly PS.n
+  -> new_seq:PS.lpoly PS.n 
+  -> spec_seq:PS.lpoly PS.n
+  -> z:zq
+  -> new_j_v:zq
+  -> new_j_plus_len_v:zq
+  -> len:len_t
+  -> start:start_t len{v start + (2 * v len) <= 256}
+  -> j:U32.t{v start <= v j /\ v j < v (start +. len)}
+  -> Lemma 
+      (requires 
+        Seq.equal (Seq.slice old_seq (v start) (v j)) (Seq.slice #_ #(PS.n) spec_seq (v start) (v j)) /\                    // the first part of the range matches the spec
+        Seq.equal (Seq.slice old_seq (v j) (v start + v len)) (Seq.slice #_ #(PS.n) orig_seq (v j) (v start + v len)) /\    // the second part of the range matches original
+        Seq.equal spec_seq (S.ntt_inner_inner_func (v z) orig_seq (v len) (v start)) /\                                     // the spec is the spec
+        Seq.equal (Seq.upd (Seq.upd old_seq (v j) (v new_j_v)) (v (j +. len)) (v new_j_plus_len_v)) new_seq)                // the new seq is updated accordingly
+      (ensures Seq.equal (Seq.slice new_seq (v start) (v j + 1)) (Seq.slice #_ #(PS.n) spec_seq (v start) (v j + 1)))
+let body_inner_inner_1 new_seq spec_seq start fin = admit()
+
+let body_inner_inner h0 (z:zq) (len:len_t) (start:start_t len{v start + (2 * v len) <= 256}) (spec_res:erased (lseq PS.zq PS.n)) (res:rq) (j:U32.t{v start <= v j /\ v j < v (start +. len)}): 
+    Stack unit 
+    (requires fun h -> inv_inner_inner h0 z len start spec_res res h (U32.v j) /\ Seq.equal spec_res (S.ntt_inner_inner_func (v z) (lpoly_v h0 res)  (v len) (v start)))
+    (ensures fun h0' _ h1 -> inv_inner_inner h0 z len start spec_res res h0' (U32.v j) /\ inv_inner_inner h0 z len start spec_res res h1 (U32.v j + 1)) 
+  =
+    let h0' = ST.get () in
+    let res_j = res.(j) in
+    let res_j_plus_len = res.(j +. len) in
+    let t = mul_zq z res_j_plus_len in
+    let new_j_v = add_zq res_j t in
+    let new_j_plus_len_v = add_zq res_j (neg_zq t) in
+    let orig_seq: erased (lseq PS.zq PS.n) = lpoly_v h0 res in
+    let old_seq: erased (lseq PS.zq PS.n) = lpoly_v h0' res in
+
+    res.(j) <- new_j_v;
+    let h0'' = ST.get () in
+    let int_seq: erased (lseq PS.zq PS.n) = lpoly_v h0'' res in
+    assert (Seq.equal (Seq.upd old_seq (v j) (v new_j_v)) int_seq);
+    res.(j +. len) <- new_j_plus_len_v;
+    let h1 = ST.get () in
+    
+    assert (v j < 256);
+    let new_seq: erased (lseq PS.zq PS.n) = lpoly_v h1 res in
+    // assert (Seq.equal spec_res (S.ntt_inner_inner_func (v z) orig_seq (v len) (v start)));
+    // the first parts of the range now match the spec
+    // seq_slice_idx_lemma (v j + v len) (v start + 2 * (v len)) (v j + v len) old_seq orig_seq;
+    body_inner_inner_1 (lpoly_v h0 res) old_seq new_seq spec_res z new_j_v new_j_plus_len_v len start j;
+    admit()
+    // // assume (Seq.equal (Seq.slice (new_seq) (v start) (v j + 1)) (Seq.slice #_ #(PS.n) spec_res (v start) (v j + 1)));
+    // assume (Seq.equal (Seq.slice #_ #(PS.n) (new_seq) (v start + v len) (v j + 1 + v len)) (Seq.slice #_ #(PS.n) spec_res (v start + v len) (v j + 1 + v len)));
+
+    // // the latter parts of the range are untouched from the original
+    // assume (Seq.equal (Seq.slice #_ #(PS.n) (new_seq) (v j + 1) (v start + v len)) (Seq.slice #_ #(PS.n) (lpoly_v h0 res) (v j + 1) (v start + v len)));
+    // assume (Seq.equal (Seq.slice #_ #(PS.n) (new_seq) (v j + 1 + v len) (v start + 2 * (v len))) (Seq.slice #_ #(PS.n) (lpoly_v h0 res) (v j + 1 + v len) (v start + 2 * (v len))))
+
+// let body_inner_inner_ h0 (z:zq) (len:len_t) (start:start_t len{v start + (2 * v len) <= 256}) (spec_res:erased (lseq PS.zq PS.n)) (res:rq) (j:U32.t{v start <= v j /\ v j < v (start +. len)}): 
+//     Stack unit 
+//     (requires fun h -> inv_inner_inner h0 z len start spec_res res h (U32.v j))
+//     (ensures fun h0' _ h1 -> inv_inner_inner h0 z len start spec_res res h0' (U32.v j) /\ inv_inner_inner h0 z len start spec_res res h1 (U32.v j + 1)) 
+//   =
+//     let h0' = ST.get () in
+//     let res_j = res.(j) in
+//     let res_j_plus_len = res.(j +. len) in
+//     let t = mul_zq z res_j_plus_len in
+//     // // res[j:start+len] = res0[j:start+len]
+//     assert (Seq.equal (Seq.slice (lpoly_v h0' res) (v j) (v start + v len)) (Seq.slice (lpoly_v h0 res) (v j) (v start + v len)));
+//     seq_slice_idx_lemma #_ (v j) (v start + v len) (v j) (lpoly_v h0' res) (lpoly_v h0 res);
+//     // res[j] = res0[j]
+//     assert (Seq.index (lpoly_v h0' res) (v j) = Seq.index (lpoly_v h0 res) (v j));
+//     seq_slice_idx_lemma #_ (v j + v len) (v start + 2 * (v len)) (v j + v len) (lpoly_v h0' res) (lpoly_v h0 res);
+//     // res[j+len] = res0[j+len]
+//     assert (Seq.index (lpoly_v h0' res) (v j + v len) = Seq.index (lpoly_v h0 res) (v j + v len));
+//     ntt_inner_inner_f_ok_1 (v j) len start z res_j res_j_plus_len (tq_v h0 res) t;
+//     // // this gives us res[j] + t (in h0') = S.ntt_inner_inner_f j len start z res (in h0)
+//     ntt_inner_inner_f_ok_2 (v j + v len) len start z res_j_plus_len res_j (tq_v h0 res) t;
+//     // // This gives us res[j] - t (in h0') = S.ntt_inner_inner_f j+len len start z res (in h0)
+//     assert (v (add_zq res_j t) == S.ntt_inner_inner_f (v j) (v len) (v start) (v z) (tq_v h0' res));
+//     assert (v (add_zq res_j (neg_zq t)) == S.ntt_inner_inner_f (v j + v len) (v len) (v start) (v z) (tq_v h0' res));
+//     res.(j) <- add_zq res_j t;
+//     res.(j +. len) <- add_zq res_j (neg_zq t);
+//     add_v_lemma j len;
+//     assert (v j + v len > v j);
+//     assert (v (j +. len) > v j);
+//     assert (v (j +. len) > v j + 1);
+//     let h1 = ST.get () in
+//     assert (Seq.index (lpoly_v h1 res) (v j) == Seq.index #_ #(PS.n) spec_res (v j));
+//     assert (Seq.equal (Seq.slice (lpoly_v h1 res) (v start) (v j)) (Seq.slice #_ #(PS.n) spec_res (v start) (v j)));
+//     slice_plus_one #_ #256 #256 (lpoly_v h1 res) spec_res (v start) (v j);
+//     assert (Seq.index (lpoly_v h1 res) (v j + v len) == Seq.index #_ #(PS.n) spec_res (v j + v len));
+//     assert (Seq.equal (Seq.slice (lpoly_v h1 res) (v start + v len) (v j + v len)) (Seq.slice #_ #(PS.n) spec_res (v start + v len) (v j + v len)));
+//     slice_plus_one #_ #256 #256 (lpoly_v h1 res) spec_res (v start + v len) (v j + v len);
+//     assert (v j + v len >= v start + v len);
+//     assert (v j < v j + v len);
+//     // assume (Seq.equal (Seq.slice (lpoly_v h1 res) (v j + 1) (v start + v len)) (Seq.slice (lpoly_v h0 res) (v j + 1) (v start + v len)));
+//     // assume (Seq.equal (Seq.slice (lpoly_v h1 res) (v j + 1 + v len) (v start + 2 * (v len))) (Seq.slice (lpoly_v h0 res) (v j + 1 + v len) (v start + 2 * (v len))));
+//     // assume (v j + 1 < v start + v len);
+//     // assume (v j + 1 <= 256) in
+//     assert (v j + 1 <= v start + v len);
+//     assert (v j + 1 >= v start);
+//     assert (v j + 1 <= 256);
+//     assert (v j >= 0);
+//     assume (Seq.equal (Seq.slice (lpoly_v h1 res) (v j + 1) (v start + v len)) (Seq.slice (lpoly_v h0 res) (v j + 1) (v start + v len)));
+//     assume (Seq.equal (Seq.slice (lpoly_v h1 res) (v j + 1 + v len) (v start + 2 * (v len))) (Seq.slice (lpoly_v h0 res) (v j + 1 + v len) (v start + 2 * (v len))));
+//     assert (Seq.equal (Seq.slice (lpoly_v h1 res) (v start) (v j + 1)) (Seq.slice #_ #(PS.n) spec_res (v start) (v j + 1)));
+//     assert (Seq.equal (Seq.slice (lpoly_v h1 res) (v start + v len) (v j + 1 + v len)) (Seq.slice #_ #(PS.n) spec_res (v start + v len) (v j + 1 + v len)))
+  
+// // This should be equivalent to running the S.ntt_inner_inner
+// val ntt_inner_inner:
+//     res:rq
+//   -> len:len_t
+//   -> start:start_t len{v start + (2 * v len) <= 256}
+//   -> z:zq
+//   -> Stack unit
+//   (requires fun h ->
+//     live h res)
+//   (ensures fun h0 _ h1 -> 
+//     live h1 res /\
+//     modifies (loc res) h0 h1 /\
+//     Seq.equal
+//       (Seq.slice (lpoly_v h1 res) (v start) (v start + v len + v len))
+//       (Seq.slice (PS.tq_to_rq (S.ntt_inner_inner_func (v z) (tq_v h0 res) (v len) (v start))) (v start) (v start + v len + v len)))
+// let ntt_inner_inner res len start z =
+//   push_frame ();
+//   let h0 = ST.get () in
+//   let spec_res: erased (lseq PS.zq PS.n) = (PS.tq_to_rq (S.ntt_inner_inner_func (v z) (tq_v h0 res)  (v len) (v start))) in
+//   let spec_tq: erased (PS.tq) = (S.ntt_inner_inner_func (v z) (tq_v h0 res)  (v len) (v start)) in
+//   let loop_stop = start +. len in
+//   assert (v len <= 256);
+//   assert (v len + v start + v len <= 256);
+//   assert (v start >= 0);
+//   let inv h (j:nat) =
+//     // start_plus_len #len start;
+//     live h res /\
+//     modifies (loc res) h0 h /\
+//     j <= v start + v len /\
+//     j >= v start /\
+//     j <= 256 /\
+//     j >= 0 /\
+//     Seq.equal
+//       (Seq.slice (lpoly_v h res) j (v start + v len))
+//       (Seq.slice (lpoly_v h0 res) j (v start + v len)) /\
+//     Seq.equal
+//       (Seq.slice (lpoly_v h res) (j + v len) (v start + 2 * (v len)))
+//       (Seq.slice (lpoly_v h0 res) (j + v len) (v start + 2 * (v len))) /\
+//     Seq.equal 
+//       (Seq.slice (lpoly_v h res) (v start) j) 
+//       (Seq.slice #_ #(PS.n) spec_res (v start) j) /\
+//     Seq.equal 
+//       (Seq.slice (lpoly_v h res) (v start + v len) (v len + j))
+//       (Seq.slice #_ #(PS.n) spec_res (v start + v len) (v len + j)) in
+//   let body (j:U32.t{v start <= v j /\ v j < v loop_stop}): 
+//     Stack unit 
+//     (requires fun h -> inv h (U32.v j))
+//     (ensures fun h0 _ h1 -> inv h0 (U32.v j) /\ inv h1 (U32.v j + 1)) 
+//   =
+//     let h0' = ST.get () in
+//     let res_j = res.(j) in
+//     let res_j_plus_len = res.(j +. len) in
+//     let t = mul_zq z res_j_plus_len in
+//     // // res[j:start+len] = res0[j:start+len]
+//     // // assert (Seq.equal (Seq.slice (lpoly_v h0' res) (v j) (v start + v len)) (Seq.slice (lpoly_v h0 res) (v j) (v start + v len)));
+//     seq_slice_idx_lemma #_ (v j) (v start + v len) (v j) (lpoly_v h0' res) (lpoly_v h0 res);
+//     // res[j] = res0[j]
+//     // assert (Seq.index (lpoly_v h0' res) (v j) = Seq.index (lpoly_v h0 res) (v j));
+//     seq_slice_idx_lemma #_ (v j + v len) (v start + 2 * (v len)) (v j + v len) (lpoly_v h0' res) (lpoly_v h0 res);
+//     // res[j+len] = res0[j+len]
+//     // assert (Seq.index (lpoly_v h0' res) (v j + v len) = Seq.index (lpoly_v h0 res) (v j + v len));
+//     ntt_inner_inner_f_ok_1 (v j) len start z res_j res_j_plus_len (tq_v h0 res) t;
+//     // // this gives us res[j] + t (in h0') = S.ntt_inner_inner_f j len start z res (in h0)
+//     ntt_inner_inner_f_ok_2 (v j + v len) len start z res_j_plus_len res_j (tq_v h0 res) t;
+//     // // This gives us res[j] - t (in h0') = S.ntt_inner_inner_f j+len len start z res (in h0)
+//     assert (v (add_zq res_j t) == S.ntt_inner_inner_f (v j) (v len) (v start) (v z) (tq_v h0' res));
+//     assert (v (add_zq res_j (neg_zq t)) == S.ntt_inner_inner_f (v j + v len) (v len) (v start) (v z) (tq_v h0' res));
+//     res.(j) <- add_zq res_j t;
+//     res.(j +. len) <- add_zq res_j (neg_zq t);
+//     assert (v j + v len > v j);
+//     assert (v (j +. len) > v j);
+//     assert (v (j +. len) > v j + 1);
+//     let h1 = ST.get () in
+//     // assert (Seq.index (lpoly_v h1 res) (v j) == Seq.index #_ #(S.n) spec_res (v j));
+//     // assert (Seq.equal (Seq.slice (lpoly_v h1 res) (v start) (v j)) (Seq.slice #_ #(S.n) spec_res (v start) (v j)));
+//     // slice_plus_one #_ #256 #256 (lpoly_v h1 res) spec_res (v start) (v j);
+//     // // assert (Seq.index (lpoly_v h1 res) (v j + v len) == Seq.index #_ #(S.n) spec_res (v j + v len));
+//     // // assert (Seq.equal (Seq.slice (lpoly_v h1 res) (v start + v len) (v j + v len)) (Seq.slice #_ #(S.n) spec_res (v start + v len) (v j + v len)));
+//     // slice_plus_one #_ #256 #256 (lpoly_v h1 res) spec_res (v start + v len) (v j + v len);
+//     assert (v j + v len >= v start + v len);
+//     assert (v j < v j + v len);
+//     // assume (Seq.equal (Seq.slice (lpoly_v h1 res) (v j + 1) (v start + v len)) (Seq.slice (lpoly_v h0 res) (v j + 1) (v start + v len)));
+//     // assume (Seq.equal (Seq.slice (lpoly_v h1 res) (v j + 1 + v len) (v start + 2 * (v len))) (Seq.slice (lpoly_v h0 res) (v j + 1 + v len) (v start + 2 * (v len))));
+//     // assume (v j + 1 < v start + v len);
+//     // assume (v j + 1 <= 256) in
+//     assert (v j + 1 <= v start + v len);
+//     assert (v j + 1 >= v start);
+//     assert (v j + 1 <= 256);
+//     assert (v j >= 0);
+//     assume (Seq.equal (Seq.slice (lpoly_v h1 res) (v j + 1) (v start + v len)) (Seq.slice (lpoly_v h0 res) (v j + 1) (v start + v len)));
+//     assume (Seq.equal (Seq.slice (lpoly_v h1 res) (v j + 1 + v len) (v start + 2 * (v len))) (Seq.slice (lpoly_v h0 res) (v j + 1 + v len) (v start + 2 * (v len))));
+//     assert (Seq.equal (Seq.slice (lpoly_v h1 res) (v start) (v j + 1)) (Seq.slice #_ #(PS.n) spec_res (v start) (v j + 1)));
+//     assert (Seq.equal (Seq.slice (lpoly_v h1 res) (v start + v len) (v j + 1 + v len)) (Seq.slice #_ #(PS.n) spec_res (v start + v len) (v j + 1 + v len))) in
+//   admit()
+//   // Lib.Loops.for start loop_stop inv body;
+//   // pop_frame ()
+
+
+// let is_len_t (l:size_t) = (v l = 2 || v l = 4 || v l = 8 || v l = 16 || v l = 32 || v l = 64 || v l = 128)
+
+// val k_lt_128:
+//     (len:len_t)
+//   -> (start:start_t len)
+//   -> Lemma (ensures v ((128ul /. len) +. (start /. (2ul *. len))) < 128)
+// let k_lt_128 len start = ()
+
+// val start_lte_256:
+//     #i:size_t{v i < 7} 
+//   -> len:len_t
+//   -> s_i:size_t
+//   -> Lemma 
+//     (requires len = (128ul >>. i) /\ s_i <. (1ul <<. i)) 
+//     (ensures v (2ul *. (1ul <<. i) *. (128ul >>. i)) <= 256)
+// let start_lte_256 #i len s_i = ()
+// val start_divisible_by_len:
+//     #i:size_t{v i < 7} 
+//   -> len:len_t
+//   -> s_i:size_t
+//   -> Lemma 
+//     (requires len = (128ul >>. i) /\ s_i <. (1ul <<. i) /\ len <> 0ul) 
+//     (ensures v (2ul *. s_i *. len) % v (2ul *. len) = 0)
+// let start_divisible_by_len #i len s_i = ()
+
+// val ntt_outer_inner:
+//     res:rq
+//   -> zeta_table:lbuffer zq 128ul
+//   -> i:size_t{v i < 7}
+//   -> Stack unit
+//   (requires fun h ->
+//     live h res /\
+//     live h zeta_table /\
+//     is_zeta_table zeta_table h)
+//   (ensures fun h0 _ h1 ->
+//     assume (is_len_t (128ul >>. i));
+//     let len:len_t = 128ul >>. i in
+//     live h1 res /\
+//     modifies (loc res) h0 h1 /\
+//     PS.tq_eq (tq_v h1 res) (S.ntt_outer_inner (tq_v h0 res) (v len) 0))
+// let ntt_outer_inner res zeta_table i =
+//   // Start goes from 0->2^8
+//   // Increments by 2*len each time, say len=2^(7-i)
+//   // # of loops is 2^8 / (2*2^(7-i)) = 2^i = 1 <<. i
+//   assume(is_len_t (128ul >>. i));
+//   let h0 = ST.get () in
+//   let len:len_t = 128ul >>. i in
+//   let loop_iters = 1ul <<. i in
+//   let spec_res: erased _ = PS.tq_to_rq (S.ntt_outer_inner (tq_v h0 res) (v len) 0) in
+//   let inv h (i:nat) =
+//     live h res /\
+//     live h zeta_table /\
+//     i <= v loop_iters /\
+//     is_zeta_table zeta_table h /\
+//     Seq.equal
+//       (Seq.slice #_ #256 (lpoly_v h res) 0 (i * 2 * (v len)))
+//       (Seq.slice #_ #256 spec_res 0 (i * 2 * (v len)))
+//     in
+//   let body (s_i:size_t{v s_i >= 0 /\ v s_i < v loop_iters}): 
+//     Stack unit 
+//     (requires fun h -> inv h (v i))
+//     (ensures fun h0 _ h1 -> inv h0 (v i) /\ inv h1 (v i + 1)) 
+//   =
+//     // Max value: 2 * 2^i * 2^(7-i) = 2^8 = 256
+//     start_lte_256 #i len s_i;
+//     start_divisible_by_len #i len s_i;
+//     let start:start_t len = 2ul *. len *. s_i in
+//     k_lt_128 len start;
+//     let k = (128ul /. len) +. (start /. (2ul *. len)) in
+//     let zeta = index_zeta_table k zeta_table in
+//     ntt_inner_inner res len start zeta in
+//   Lib.Loops.for 0ul loop_iters inv body
+
+
+// val ntt:
+//     f:rq
+//   -> res:rq
+//   -> zeta_table:lbuffer zq 128ul
+//   -> Stack unit
+//   (requires fun h ->
+//     live h f /\ live h res /\
+//     live h zeta_table /\
+//     disjoint f res
+//   )
+//   (ensures fun h0 _ h1 ->
+//     live h1 f /\
+//     live h1 res /\
+//     disjoint f res /\
+//     modifies (loc res) h0 h1 /\
+//     PS.tq_eq (tq_v h1 res) (S.ntt (lpoly_v h0 f))
+//    )
+// let ntt f res zeta_table =
+//   push_frame ();
+//   let h0 = ST.get () in
+//   precomp_zeta zeta_table;
+//   let inv_inner_inner (len:len_t) (start:start_t len) (z:zq) h (j':nat) =
+//     let j:nat = v start + j' in
+//     let spec_tq = (S.ntt_inner_inner (v z) (tq_v h f) j (v len) (v start)) in
+//     // let first_part_spec = Seq.slice (S.tq_to_rq spec_tq) (v start) (j + 1) in
+//     // let first_part_impl = Seq.slice (lpoly_v h res) (v start) (j + 1) in
+//     // let second_part_spec = Seq.slice (S.tq_to_rq spec_tq) (v start + v len) (v len + j + 1) in
+//     // let second_part_impl = Seq.slice (lpoly_v h res) (v start + v len) (v len + j + 1) in
+//     j' <= v len /\
+//     live h f /\ live h res /\ modifies (loc res) h0 h /\ j' < v len /\
+//     Seq.equal 
+//       (Seq.slice (lpoly_v h res) (v start) (j + 1)) 
+//       (Seq.slice (PS.tq_to_rq spec_tq) (v start) (j + 1)) /\
+//     Seq.equal 
+//       (Seq.slice (lpoly_v h res) (v start + v len) (v len + j + 1)) 
+//       (Seq.slice (PS.tq_to_rq spec_tq) (v start + v len) (v len + j + 1)) in
+//   let body_inner_inner (len:len_t) (start:start_t len) (z:zq) (j':size_t{v j' < v len}): 
+//     Stack unit 
+//     (requires (fun h -> inv_inner_inner len start z h (v j'))) 
+//     (ensures (fun h0 _ h1 -> inv_inner_inner len start z h0 (v j') /\ inv_inner_inner len start z h1 (v j' + 1))) 
+//   =
+//     let h0 = ST.get () in
+//     let j = start +. j' in
+//     let t = mul_zq z f.(j +. len) in
+//     start_plus_len #len start;
+//     assert (v j < 256);
+//     res.(j) <- add_zq f.(j) t;
+//     res.(j +. len) <- add_zq f.(j) (neg_zq t) in
+//   let inv_outer_inner (#i:size_t{i <. 7ul}) (len:len_t) h (i':nat) =
+//     assert (i' < v (1ul <<. i));
+//     start_t_lemma #i (u32 i');
+//     let start:S.start_t (v len) = 2 * (v len) * i' in
+//     let spec_tq = S.ntt_outer_inner (tq_v h f) (v len) start in
+//     live h f /\ live h res /\ modifies (loc res) h0 h /\ i' < (pow2 (v i)) /\
+//     // After each loop iteration, we should have the next 2*len elements match spec (from calling inner_inner)
+//     Seq.equal 
+//       (Seq.slice (PS.tq_to_rq spec_tq) 0 (start + 2 * len))
+//       (Seq.slice (PS.tq_to_rq (tq_v h res)) 0 (start + 2 * len)) in
+//   let body_outer_inner #i (len:len_t) (i':size_t{i' <. (1ul <<. i)}): 
+//     Stack unit 
+//     (requires (fun h -> inv_outer_inner #i len h (v i'))) 
+//     (ensures (fun h0 _ h1 -> inv_outer_inner #i len h0 (v i') /\ inv_outer_inner #i len h1 (v i' + 1))) 
+//   = 
+//     assume (2ul *. len *. i' <. 256ul);
+//     let start:start_t len = 2ul *. len *. i' in
+//     let k = (128ul /. len) +. (start /. (2 *. len)) in
+//     let z = zeta_table.(k) in
+//     Lib.Loops.for 0ul len (inv_inner_inner len start z) (body_inner_inner start z len) in
+//   let inv_outer h (i:nat) =
+//     live h f /\ live h res /\ modifies (loc res) h0 h /\ i < 7 /\
+//     Seq.equal (PS.tq_to_rq (S.ntt_outer_intermediate (tq_v h f) i)) (PS.tq_to_rq (tq_v h res)) in
+//   let body_outer (i:size_t):
+//     Stack unit
+//     (requires (fun h -> inv_outer h (v i)))
+//     (ensures (fun h0 _ h1 -> inv_outer h0 (v i) /\ inv_outer h1 (v i + 1)))
+//   =
+//     let len = 128ul >>. i in
+//     Lib.Loops.for 0ul (1ul <<. i) (inv_outer_inner #i len) (body_outer_inner #i len) in
+//   Lib.Loops.for 0ul 7ul inv_outer body_outer;
+//   pop_frame ()
+
+
+// val intt:
+//     #deg: size_t
+//   -> a:rq
+//   -> res:rq
+//   -> Stack unit
+//   (requires fun h ->
+//     live h a /\ live h res /\
+//     disjoint a res
+//   )
+//   (ensures fun h0 _ h1 ->
+//     live h1 a /\
+//     live h1 res /\
+//     disjoint a res /\
+//     modifies (loc res) h0 h1 /\
+//     Seq.equal (lpoly_v h1 res) (S.intt (tq_v h0 a))
+//    )
