code/mlkem/Hacl.Spec.MLkem.NTT.fst
@@ -1,0 +1,288 @@
+module Hacl.Spec.MLkem.NTT
+open FStar.Mul
+open FStar.Seq
+unfold let max = FStar.Math.Lib.max
+
+open Lib.IntTypes
+open Lib.Sequence
+open Lib.NatMod
+open Hacl.Spec.MLkem.Poly
+
+#reset-options "--z3rlimit 50 --fuel 0 --ifuel 0"
+
+let zeta = 17
+let bit7 = lseq bool 7
+
+let bitrev7 (bits:bit7): bit7 =
+  createi 7 (fun i -> index bits (6 - i))
+
+let bit (b:bool): b:nat{b = 0 || b = 1} = if b then 1 else 0
+
+let bit7_v (bits:bit7): r:nat{r < 128} =
+  let r0 = bit (index bits 0) in 
+  let r1 = bit (index bits 1) in
+  let r2 = bit (index bits 2) in
+  let r3 = bit (index bits 3) in
+  let r4 = bit (index bits 4) in
+  let r5 = bit (index bits 5) in
+  let r6 = bit (index bits 6) in
+  r0 + 2 * r1 + 4 * r2 + 8 * r3 + 16 * r4 + 32 * r5 + 64 * r6
+
+let bitrev_ok (bits:bit7): Lemma 
+  (requires True) 
+  (ensures (
+    let rev = bitrev7 bits in
+    forall (i:nat{ i < 7 }). (index bits i = index rev (6 - i))
+  )) = ()
+
+let get_bit (bits:nat{ bits < 128}) (i:nat{i < 7}): b:nat{b = 0 || b = 1 } =
+  bits / (pow2 i) % 2
+
+let bitsequence (i:nat{ i < 128}): bit7 =
+  createi 7 (fun j -> (get_bit i j) = 1)
+
+let bitrev7_int (bits:nat{bits < 128}): result:nat{result < 128} =
+  bit7_v (bitrev7 (bitsequence bits))
+
+// Types specifying the possible values of the length and start parameters
+type len_t = l:nat{l = 2 || l = 4 || l = 8 || l = 16 || l = 32 || l = 64 || l = 128}
+type start_t (len:len_t) = s:nat{s % (2*len) = 0 && s < 256}
+
+// These just convert between the two representations of polynomials, such that 
+// f[2i] = p[i][0] and f[2i+1] = p[i][1] (does not do the actual NTT)
+// let rq_to_tq (f:rq): tq =
+//   createi 128 (fun i ->
+//     let f0 = index f (2 * i) in
+//     let f1 = index f (2 * i + 1) in
+//     let p: lpoly 2 = cons f0 (cons f1 empty) in
+//     p
+//   )
+// let tq_to_rq (f:tq): rq =
+//   createi 256 (fun i ->
+//     let p = index f (i / 2) in
+//     if i % 2 = 0 then
+//       index p 0
+//     else
+//       index p 1
+//   )
+// let tq_eq (f g: tq) = 
+//   let f_rq = tq_to_rq f in
+//   let g_rq = tq_to_rq g in
+//   Seq.equal f_rq g_rq
+
+val ntt_inner_inner:
+    z:zq
+  -> f:tq
+  -> j:nat
+  -> len:len_t
+  -> start:start_t len
+  -> Tot (tq) (decreases (start + len) - j)
+let rec ntt_inner_inner z f j len start: tq =
+  // for j <- start; j < start + len; j++
+  if j < (start + len) then
+    // t <- zeta * f_hat[j+ len]
+    let t = mul_zq z (index_tq f (j + len)) in
+    let f_j = index_tq f j in
+    // f_hat[j + len] <- f_hat[j] - t
+    let f_upd = upd_tq f (j + len) (add_zq f_j (neg_zq t)) in
+    // f_hat[j] <- f_hat[j] + t
+    let f_upd_upd = upd_tq f_upd j (add_zq f_j t) in
+    ntt_inner_inner z f_upd_upd (j + 1) len start
+  else
+    f
+
+val ntt_inner_inner_f (j:nat{j < 256}) (len:len_t) (start:start_t len) (z:zq) (f:tq): zq
+let ntt_inner_inner_f j len start z f =
+    if j < start || j >= start + 2 * len then
+      index_tq f j
+    else if j >= start && j < start + len then
+      let t = mul_zq z (index_tq f (j + len)) in
+      add_zq (index_tq f j) t
+    else
+      let t = mul_zq z (index_tq f j) in
+      add_zq (index_tq f (j - len)) (neg_zq t)
+
+
+val ntt_inner_inner_func:
+    z:zq 
+  -> f:tq 
+  -> len:len_t
+  -> start:start_t len
+  -> tq
+let ntt_inner_inner_func z f len start = 
+  let rq_rep = createi #zq 256 (fun j -> ntt_inner_inner_f j len start z f) in rq_to_tq rq_rep
+
+// val ntt_inner_inner_func_ok: 
+//     z:zq
+//   -> f:tq
+//   -> len:len_t
+//   -> start:start_t len
+//   -> Lemma (ensures ntt_inner_inner z f start len start = ntt_inner_inner_func z f len start)
+// let ntt_inner_inner_func_ok z f len start = ()
+
+val zeta_to_k:
+    k:nat{k < 128}
+  -> zq
+let zeta_to_k k = pow_mod #q zeta k
+let test = 
+  let zeta_0 = pow_mod #q zeta 0 in
+  pow_mod_def #q zeta 0;
+  lemma_pow_mod #q zeta 0;
+  lemma_pow0 zeta;
+  assert (zeta_0 = 1);
+  ()
+
+val zeta_to_k_pos_lemma: (k:nat{k > 0 && k < 128}) -> Lemma (requires True) (ensures (zeta_to_k k = mul_zq (zeta_to_k (k - 1)) zeta))
+let zeta_to_k_pos_lemma k = 
+  pow_mod_def #q zeta k;
+  lemma_pow_mod #q zeta k;
+  lemma_pow_unfold zeta k;
+  assert (pow zeta k % q = zeta_to_k k);
+  assert (zeta * pow zeta (k - 1) % q = zeta_to_k k);
+  lemma_pow_mod #q zeta (k - 1);
+  assert (pow zeta (k - 1) % q = zeta_to_k (k - 1));
+  ()
+
+val ntt_outer_inner_body:
+    f:tq
+  -> len:len_t
+  -> start:start_t len
+  -> k:nat{k < 128}
+  -> tq
+let ntt_outer_inner_body f len start k = 
+  // zeta <- Zeta ^ (BitRev7(k)) mod q
+  let z = pow_mod #q zeta (bitrev7_int k) in
+  let f_upd = ntt_inner_inner z f start len start in
+  f_upd
+
+val ntt_outer_inner:
+    f:tq
+  -> len:len_t
+  -> start:start_t len
+  -> Tot (tq) (decreases (256 - 2 * len) - start)
+let rec ntt_outer_inner f len start =
+  let k = (128 / len) + (start / (2 * len)) in
+  let f_upd:tq = ntt_outer_inner_body f len start k in
+  if start + 2 * len >= 256 then 
+    f_upd
+  else
+    ntt_outer_inner f_upd len (start + 2 * len)
+
+val ntt_outer:
+    len:len_t
+  -> f:tq
+  -> Tot tq (decreases len)
+let rec ntt_outer len f =
+  let f_upd = ntt_outer_inner f len 0 in
+  if len = 2 then
+    f_upd
+  else
+    ntt_outer (len / 2) f_upd
+
+val len_t_lemma: (i:nat{i < 7}) -> 
+  Lemma (ensures pow2 i = 2 || pow2 i = 4 || pow2 i = 8 || pow2 i = 16 || pow2 i = 32 || pow2 i = 64)
+let len_t_lemma i = admit()
+
+val ntt_outer_intermediate:
+    f:tq
+  -> i:nat{i < 7}
+  -> Tot tq (decreases i)
+let rec ntt_outer_intermediate f i =
+  len_t_lemma (6-i);
+  let len:len_t = 128 / (pow2 (6-i)) in
+  let f_upd = ntt_outer_inner f len 0 in
+  if i = 0 then
+    f_upd
+  else
+    ntt_outer_intermediate f_upd (i-1)
+
+// val ntt_outer_int_ok: 
+//     f:tq
+//   -> Lemma (requires True) (ensures (ntt_outer 128 f = ntt_outer_intermediate f 6))
+// let ntt_outer_int_ok f =
+//   assert (ntt_outer 2 f = ntt_outer_intermediate f 0);
+//   ()
+
+let ntt (f:rq): tq =
+  let ntt_image = ntt_outer 128 (rq_to_tq f) in 
+  ntt_image
+
+val intt_inner_inner:
+    z:zq
+  -> f:tq
+  -> j:nat
+  -> len:len_t
+  -> start:start_t len
+  -> Tot (tq) (decreases (start + len) - j)
+let rec intt_inner_inner z f j len start: tq =
+  // for j <- start; j < start + len; j++
+  if j < (start + len) then
+    // t <- zeta * f_hat[j+ len]
+    let t = (index_tq f j) in 
+    // f[j] <- t + f[j+len]
+    let f_j = add_zq t (index_tq f (j + len)) in
+    let f_upd = upd_tq f j f_j in
+    // f[j+len] <- zeta * (f[j+len] - t)
+    let f_j_len = mul_zq z (add_zq (index_tq f (j + len)) (neg_zq t)) in
+    let f_upd_upd = upd_tq f_upd (j + len) f_j_len in
+    intt_inner_inner z f_upd_upd (j + 1) len start
+  else
+    f
+
+val intt_outer_inner_body:
+    f:tq
+  -> len:len_t
+  -> start:start_t len
+  -> k:nat{k < 128}
+  -> tq
+let intt_outer_inner_body f len start k =
+  // zeta <- Zeta ^ (BitRev7(k)) mod q
+  let z = pow_mod #q zeta (bitrev7_int k) in
+  let f_upd = intt_inner_inner z f start len start in
+  f_upd
+
+
+val intt_outer_inner:
+    f:tq
+  -> len:len_t
+  -> start:start_t len
+  -> Tot tq (decreases (256 - 2 * len) - start)
+let rec intt_outer_inner f len start =
+  let k = (256 / len) - (start / (2 * len)) - 1 in
+  // zeta <- Zeta ^ (BitRev7(k)) mod q
+  let z = pow_mod #q zeta (bitrev7_int k) in
+  let f_upd = intt_outer_inner_body f len start k in
+  if start + 2 * len >= 256 then
+    f_upd
+  else
+    intt_outer_inner f_upd len (start + 2 * len)
+
+val intt_outer:
+    len:len_t
+  -> f:tq
+  -> Tot tq (decreases (128 - len))
+let rec intt_outer len f =
+  let f_upd = intt_outer_inner f len 0 in
+  if len = 128 then
+    f_upd
+  else
+    intt_outer (len * 2) f_upd
+
+val intt:
+    f:tq
+  -> rq
+let intt f =
+  let intt_image = intt_outer 128 f in 
+  let unscaled_intt = tq_to_rq intt_image in
+  scalar_mul unscaled_intt 3303
+
+// NTT multiplication specification
+// i-th coordinate in Tq of the product hat(h) = hat(f) x_Tq hat(g) is given by:
+//    hat(h)[2i] + hat(h)[2i+1] = (hat(f)[2i]+hat(f)[2i+1]X) * (hat(g)[2i]+hat(g)[2i+1]X) mod (X^2 - zeta^(2 BitRev_7(i)+1))
+
+// index f i should yield an lpoly 2 which is equivalent to f[2i]+f[2i+1]X
+// ntt_mul_base calculates the product of two lpoly 2 with modulus X^2 - gamma
+let ntt_mul_base (a b:lpoly 2) (gamma: zq): lpoly 2 =
+  let c0 = add_zq (mul_zq (index a 0) (index b 0)) (mul_zq gamma (mul_zq (index a 1) (index b 1))) in
+  let c1 = add_zq (mul_zq (index a 0) (index b 1)) (mul_zq (index a 1) (index b 0)) in
+  cons c0 (cons c1 empty)
